Tidy up type signatures

Move.thy
@@ -8,24 +8,26 @@ datatype ('time, 'node) operation
 datatype ('time, 'node) log_op
   = LogMove (log_time: 'time) (old_parent: \<open>'node option\<close>) (new_parent: 'node) (log_child: 'node)
 
+type_synonym ('t, 'n) state = \<open>('t, 'n) log_op list \<times> ('n \<times> 'n) set\<close>
+
 (*
 datatype 'node tree   
   = Node 'node \<open>'node tree fset\<close>
 *)
 
-definition get_parent :: \<open>'n \<Rightarrow> ('n \<times> 'n) set \<Rightarrow> 'n option\<close> where
-  \<open>get_parent ch tree \<equiv>
-     if \<exists>!parent. (parent, ch) \<in> tree then
-       Some (THE parent. (parent, ch) \<in> tree)
+definition get_parent :: \<open>('n \<times> 'n) set \<Rightarrow> 'n \<Rightarrow> 'n option\<close> where
+  \<open>get_parent tree child \<equiv>
+     if \<exists>!parent. (parent, child) \<in> tree then
+       Some (THE parent. (parent, child) \<in> tree)
      else None\<close>
 
 inductive ancestor :: "('n \<times> 'n) set \<Rightarrow> 'n \<Rightarrow> 'n \<Rightarrow> bool" where
   "\<lbrakk>(parent, child) \<in> tree\<rbrakk> \<Longrightarrow> ancestor tree parent child" |
   "\<lbrakk>(parent, child) \<in> tree; ancestor tree anc parent\<rbrakk> \<Longrightarrow> ancestor tree anc child"
 
-fun apply_op :: \<open>('t, 'n) operation \<times> ('n \<times> 'n) set \<Rightarrow> ('t, 'n) log_op \<times> ('n \<times> 'n) set\<close> where
-  \<open>apply_op (Move t newp c, tree) =
-     (LogMove t (get_parent c tree) newp c,
+fun do_op :: \<open>('t, 'n) operation \<times> ('n \<times> 'n) set \<Rightarrow> ('t, 'n) log_op \<times> ('n \<times> 'n) set\<close> where
+  \<open>do_op (Move t newp c, tree) =
+     (LogMove t (get_parent tree c) newp c,
       if ancestor tree c newp then tree
       else {(p', c') \<in> tree. c' \<noteq> c} \<union> {(newp, c)})\<close>
 
@@ -34,56 +36,59 @@ fun undo_op :: \<open>('t, 'n) log_op \<times> ('n \<times> 'n) set \<Rightarrow
   \<open>undo_op (LogMove t (Some oldp) newp c, tree) =
      {(p', c') \<in> tree. c' \<noteq> c} \<union> {(oldp, c)}\<close>
 
-fun reapply_op :: \<open>('t, 'n) log_op \<Rightarrow> ('t, 'n) log_op list \<times> ('n \<times> 'n) set \<Rightarrow> ('t, 'n) log_op list \<times> ('n \<times> 'n) set\<close> where
-  \<open>reapply_op (LogMove t _ p c) (ops, tree) =
-     (let (op2, tree2) = apply_op (Move t p c, tree)
+fun redo_op :: \<open>('t, 'n) log_op \<Rightarrow> ('t, 'n) state \<Rightarrow> ('t, 'n) state\<close> where
+  \<open>redo_op (LogMove t _ p c) (ops, tree) =
+     (let (op2, tree2) = do_op (Move t p c, tree)
       in (op2 # ops, tree2))\<close>
 
-fun add_op :: \<open>('t::{linorder}, 'n) operation \<Rightarrow> ('n \<times> 'n) set \<Rightarrow> ('t, 'n) log_op list \<Rightarrow> ('t, 'n) log_op list \<times> ('n \<times> 'n) set\<close> where
-  \<open>add_op op1 tree1 [] =
-     (let (op2, tree2) = apply_op (op1, tree1)
+fun interp_op :: \<open>('t::{linorder}, 'n) operation \<Rightarrow> ('t, 'n) state \<Rightarrow> ('t, 'n) state\<close> where
+  \<open>interp_op op1 ([], tree1) =
+     (let (op2, tree2) = do_op (op1, tree1)
       in ([op2], tree2))\<close> |
-  \<open>add_op op1 tree1 (logop # ops) =
+  \<open>interp_op op1 (logop # ops, tree1) =
      (if move_time op1 < log_time logop
-      then reapply_op logop (add_op op1 (undo_op (logop, tree1)) ops)
-      else let (op2, tree2) = apply_op (op1, tree1) in (op2 # ops, tree2))\<close>
+      then redo_op logop (interp_op op1 (ops, undo_op (logop, tree1)))
+      else let (op2, tree2) = do_op (op1, tree1) in (op2 # ops, tree2))\<close>
+
+definition interp_ops :: \<open>('t::{linorder}, 'n) operation list \<Rightarrow> ('t, 'n) log_op list \<times> ('n \<times> 'n) set\<close> where
+  \<open>interp_ops ops \<equiv> foldl (\<lambda>state op. interp_op op state) ([], {}) ops\<close>
 
 lemma get_parent_None:
   assumes \<open>\<nexists>p. (p, c) \<in> tree\<close>
-  shows \<open>get_parent c tree = None\<close>
+  shows \<open>get_parent tree c = None\<close>
 by (meson assms get_parent_def)
 
 lemma get_parent_Some:
   assumes \<open>(p, c) \<in> tree\<close>
     and \<open>\<And>x. (x, c) \<in> tree \<Longrightarrow> x = p\<close>
-  shows \<open>get_parent c tree = Some p\<close>
+  shows \<open>get_parent tree c = Some p\<close>
 proof -
   have \<open>\<exists>!parent. (parent, c) \<in> tree\<close>
     using assms by metis
   hence \<open>(THE parent. (parent, c) \<in> tree) = p\<close>
     using assms(2) by fastforce
-  thus \<open>get_parent c tree = Some p\<close>
+  thus \<open>get_parent tree c = Some p\<close>
     using assms get_parent_def by metis
 qed
 
-lemma apply_undo_inv:
+lemma do_undo_op_inv:
   assumes \<open>\<And>x. (x, c) \<in> tree \<Longrightarrow> x = oldp\<close>
-  shows \<open>undo_op (apply_op (Move t p c, tree)) = tree\<close>
+  shows \<open>undo_op (do_op (Move t p c, tree)) = tree\<close>
 proof(cases \<open>\<exists>par. (par, c) \<in> tree\<close>)
   case True
   hence 1: \<open>(oldp, c) \<in> tree\<close>
     using assms by blast
-  hence 2: \<open>get_parent c tree = Some oldp\<close>
+  hence 2: \<open>get_parent tree c = Some oldp\<close>
     using assms get_parent_Some by metis
-  moreover have \<open>\<And>p' c'. (p', c') \<in> tree \<Longrightarrow> (p', c') \<in> undo_op (apply_op (Move t p c, tree))\<close>
+  moreover have \<open>\<And>p' c'. (p', c') \<in> tree \<Longrightarrow> (p', c') \<in> undo_op (do_op (Move t p c, tree))\<close>
     using assms calculation by auto
-  moreover have \<open>\<And>p' c'. (p', c') \<in> undo_op (apply_op (Move t p c, tree)) \<Longrightarrow> (p', c') \<in> tree\<close>
+  moreover have \<open>\<And>p' c'. (p', c') \<in> undo_op (do_op (Move t p c, tree)) \<Longrightarrow> (p', c') \<in> tree\<close>
     using 1 2 by (cases \<open>ancestor tree c p\<close>, auto)
   ultimately show ?thesis
     by (meson pred_equals_eq2)
 next
   case no_old_parent: False
-  hence \<open>get_parent c tree = None\<close>
+  hence \<open>get_parent tree c = None\<close>
     using assms get_parent_None by metis
   moreover have \<open>{(p', c') \<in> tree. c' \<noteq> c} = tree\<close>
     using no_old_parent by fastforce
@@ -91,37 +96,5 @@ next
     by auto
   ultimately show ?thesis by simp
 qed
-
-
-find_consts name: List
-
-fun find_position :: \<open>('time::{linorder}, 'node) log_op list \<Rightarrow> 'time \<Rightarrow>
-                        ('time, 'node) log_op list \<times> ('time, 'node) log_op list\<close> where
-  \<open>find_position ls t =
-     (List.filter (\<lambda>x. timestamp x < t) ls, List.filter (\<lambda>x. timestamp x > t) ls)\<close>
-
-fun undo_all :: \<open>('time, 'node) log_op list \<Rightarrow> ('node option \<times> 'node) set \<Rightarrow> ('node option \<times> 'node) set\<close> where
-  \<open>undo_all [] tree = tree\<close> |
-  \<open>undo_all (x#xs) tree = undo_all xs (undoop x tree)\<close>
-
-fun interpret_oplist :: \<open>('node option \<times> 'node) set \<Rightarrow> ('time::{linorder},'node) operation \<Rightarrow> ('time, 'node) log_op list  \<Rightarrow>
-                            ('node option \<times> 'node) set \<times> ('time, 'node) log_op list\<close> where
-  \<open>interpret_oplist forest (Move t p c) log =
-     (let (ls, gs) = find_position log t;
-          nt       = undo_all gs forest
-      in undefined)\<close>
-
-(*fun find_position :: \<open>('time, 'node) log_op list \<Rightarrow> 'time \<Rightarrow>
-
-fun update_tree :: \<open>'node tree \<Rightarrow> ('time,'node) operation \<Rightarrow> 'node tree\<close> where
-  \<open>update_tree tree oper = tree\<close>
-
-fun interpret_oplist :: \<open>'node tree \<Rightarrow> ('time::{linorder},'node) operation \<Rightarrow> ('time, 'node) log_op list  \<Rightarrow>
-                            'node tree \<times> ('time, 'node) log_op list\<close> where
-  \<open>interpret_oplist tree (Move t p c) [] = (update_tree tree (Move t p c), [UndoMove t None p c])\<close>
-| \<open>interpret_oplist tree (Move t p c) ((UndoMove t' p' c') # ops) =
-    if t < t' then
-      (UndoMove t' p' c') # interp_oplist (undo_op (UndoMove t' p' c') tree) (Move t p c) ops
-    else *)
 
 end
